## 4.1 Gamma function
Gamma function 4:1:1
$$
\boxed{
\Gamma(n) = \int_{0}^{\infty} e^{-x}x^{n-1} \, \mathrm{d}x
}
$$

$$
\Gamma(1) = \int_{0}^{\infty} e^{-x} \, \mathrm{d}x = 1 
$$

$$
\Gamma(n+1) = \int_{0}^{\infty} e^{-x}x^{n} \, \mathrm{d}x 
$$
$$
\Gamma(n+1) = -e^{-x}x^{n} \Big|_{0}^{\infty} + \int_{0}^{\infty} e^{-x}nx^{n-1} \, \mathrm{d}x 
$$
$$
\Gamma(n+1) = n\Gamma(n)
$$


### 
$$
\int_{0}^{\infty} e^{-x^{3}} \, \mathrm{d}x 
$$
$$
y = x^{3} , dx = \frac{1}{3} y^{-\frac{2}{3}} dy
$$

$$
I = \int_{0}^{\infty} e^{-y} \frac{1}{3}y^{- \frac{2}{3}} \, \mathrm{d}y =
\frac{1}{3} \Gamma\left( \frac{1}{3} \right) = \Gamma\left( \frac{4}{3} \right)
$$

$$
\boxed{
\int_{0}^{\infty} e^{-x^{3}} \, \mathrm{d}x = \Gamma\left( \frac{4}{3} \right)
}
$$

## 4.2 Wallisâ€™ Integral and the Beta Function

Wallis integral
$$
\boxed{
I(n) = \int_{0}^{1} (x-x^{2})^{n} \, \mathrm{d}x 
} 
$$
$$
\begin{array}{l}
I(0) = 1 \\
I(1) = \frac{1}{6} \\
I(2) = \frac{1}{30}
\end{array}
$$

beta function 4:2:1
$$
\boxed{
B(m,n) = \int_{0}^{1} x^{m-1}(1-x)^{n-1} \, \mathrm{d}x ,
m>0, n>0.
} 
$$

The beta function is intimately related to the gamma function.

4.1.1 ${x=y^{2},dx = 2ydy}$
$$
\Gamma(n) = \int_{0}^{\infty} e^{-y^{2}} y^{2n-2}2y \, \mathrm{d}y =
2\int_{0}^{\infty} e^{-y^{2}}y^{2n-1} \, \mathrm{d}y 
$$
$$
\Gamma(m) = \int_{0}^{\infty} e^{-x^{2}} x^{2m-1} \, \mathrm{d}x 
$$
$$
\begin{align}
\Gamma(m)\Gamma(n) & = 4 \int_{0}^{\infty} e^{-x^{2}}x^{2m-1} \, \mathrm{d}x \int_{0}^{\infty} e^{-y^{2}}y^{2n-1} \, \mathrm{d}y  \\
  & = 4\int_{0}^{\infty} \int_{0}^{\infty} e^{-(x^{2}+y^{2})} x^{2m-1} y^{2n-1} \, \mathrm{d}x  \, \mathrm{d}y 
\end{align}
$$

swithc from cartesian coordinates to polar coordinates
${r^{2}=x^{2}+y^{2},x=r\cos\theta,y=r\sin\theta}$ 
the region ${0\leq x,y\leq \infty}$ is equivalent to the region ${0\leq r\leq \infty, 0\leq \theta \leq \frac{\pi}{2}}$ 
$$
\Gamma(m)\Gamma(n) =
4\int_{0}^{\frac{\pi}{2}} \int_{0}^{\infty} e^{-r^{2}} r^{2m+2n-2}\cos ^{2m-1}(\theta) \sin ^{2n-1}(\theta)  r\, \mathrm{d}r   \, \mathrm{d}\theta
$$
$$
\Gamma(m)\Gamma(n) =
\left[ 2\int_{0}^{\infty} e^{-r^{2}}r^{2(m+n)-1} \, \mathrm{d}r \right] 
\left[ 2\int_{0}^{\frac{\pi}{2}} \cos ^{2m-1}(\theta) \sin ^{2n-1}(\theta)  \, \mathrm{d}\theta \right] 
$$
$$
2\int_{0}^{\infty} e^{-r^{2}}r^{2(m+n)-1} \, \mathrm{d}r =  
\Gamma(m+n)
$$

${x=\cos ^{2}\theta , dx=-2\sin\theta \cos\theta d\theta}$
${1-x=\sin ^{2}\theta}$ 
$$
B(m,n) = \int_{0}^{1} x^{m-1}(1-x)^{n-1} \, \mathrm{d}x 
= -2 \int_{\frac{\pi}{2}}^{0} \cos ^{2m-1}(\theta) \sin ^{2n-2}(\theta)\sin(\theta)\cos(\theta) \, \mathrm{d}\theta 
$$

$$
\boxed{
B(m,n) = 2\int_{0}^{\frac{\pi}{2}} \cos ^{2m-1}(\theta) \sin ^{2n-1}(\theta)  \, \mathrm{d}\theta 
} 
$$

$$
\boxed{\Gamma(m)\Gamma(n) = \Gamma(m+n)B(m,n)} 
$$
4:2:5
$$
\boxed{B(m,n) = \frac{\Gamma(m)\Gamma(n)}{\Gamma(m+n)}} 
$$


$$
I(k) = \int_{0}^{1} (x-x^{2})^{k} \, \mathrm{d}x 
= \int_{0}^{1} x^{k}(1-x)^{k} \, \mathrm{d}x 
= B(k+1,k+1) = \frac{\Gamma(k+1)\Gamma(k+1)}{\Gamma(2k+2)}
$$

using 4:1:3
$$
I(k) = \frac{(k!)^{2}}{(2k+1)!}
$$

4:2:6
$$
\boxed{
I(n) = \int_{0}^{1} (x-x^{2})^{n} \, \mathrm{d}x =
\frac{(n!)^{2}}{(2n+1)!}.
} 
$$

#### ex  n=7
$$
\int_{0}^{1} (x-x^{2})^{7} \, \mathrm{d}x = \frac{(7!)^{2}}{15!} = 1.9425\dots \times 10^{-5}
$$

n=1/2
$$
\int_{0}^{1} \sqrt{ x-x^{2} } \, \mathrm{d}x = \frac{\left( \frac{1}{2}! \right)^{2}}{2!} = \frac{1}{2}\left( \frac{1}{2}! \right)^{2}
$$

$$
\left( \frac{1}{2}! \right) = \Gamma\left( \frac{3}{2} \right) = \int_{0}^{\infty} e^{-x}x^{3/2 - 1} \, \mathrm{d}x 
$$
$$
\Gamma\left( \frac{3}{2} \right) = \frac{1}{2}\Gamma\left( \frac{1}{2} \right)
$$
$$
\Gamma\left( \frac{1}{2} \right) = \int_{0}^{\infty} e^{-x}x^{-1/2} \, \mathrm{d}x = \sqrt{ \pi }
$$
$$
\int_{0}^{1} \sqrt{ x-x^{2} } \, \mathrm{d}x = \frac{1}{2} \left( \frac{1}{2}\Gamma\left( \frac{1}{2} \right) \right)^{2} = 
\frac{\pi}{8}
$$


$$
\Gamma(n) = (n-1)!
$$

4:2:8
$$
\boxed{
\int_{0}^{\infty} e^{-x}\sqrt{ x } \, \mathrm{d}x = \frac{1}{2}\sqrt{ \pi }
} 
$$

#### sq{-ln x}

$$
\int_{0}^{1} \sqrt{ -\ln x } \, \mathrm{d}x 
$$
let ${y=-\ln x, x = e^{-y},dx=-e^{-y}dy}$
$$
\int_{\infty}^{0} \sqrt{ y } (-e^{-y}) \, \mathrm{d}y =
\int_{0}^{\infty} e^{-y}\sqrt{ y } \, \mathrm{d}y 
$$
$$
\boxed{\int_{0}^{1} \sqrt{ -\ln x } \, \mathrm{d}x =
\frac{1}{2}\sqrt{ \pi }
} 
$$
$$
\boxed{
\int_{0}^{\infty} e^{-x}x^{-1/2} \, \mathrm{d}x =\sqrt{ \pi }
} 
$$


$$
\Gamma\left( \frac{1}{2} \right)
\Gamma\left( \frac{1}{2} \right) = 
\Gamma(1)B(1,2) = \Gamma(1) \left[ 2\int_{0}^{\pi/2}  \, \mathrm{d}\theta \right] = \pi
$$
$$
\Gamma\left( \frac{1}{2} \right) = \sqrt{ \pi }
$$

%% todo%%  pp 125

#### sq{sin x}
let ${u=\sin ^{2}x, \sin x=u^{1/2},\cos x=(1-u)^{1/2}}$ 
${x = \arcsin u^{1/2}}$
${dx = \frac{1}{2}(1-u)^{-1/2}u^{-1/2}}$ 
$$
\boxed{
\int_{0}^{\pi/2} \sqrt{ \sin x } \, \mathrm{d}x =  
\int_{0}^{\pi/2} \sqrt{ \cos x } \, \mathrm{d}x =  
\frac{1}{2}B\left( \frac{3}{4}, \frac{1}{2} \right) = 
\frac{{\Gamma\left( \frac{3}{4} \right)\Gamma\left( \frac{1}{2} \right)}}{2\Gamma\left( \frac{5}{4} \right)}
} 
$$


$$
\boxed{ 
\int_{0}^{\pi/2} \frac{1}{\sqrt{ \sin x\cos x }} \, \mathrm{d}x 
= \frac{\Gamma^{2}\left( \frac{1}{4} \right)}{2\Gamma\left( \frac{1}{2} \right)}
= \frac{\Gamma^{2}\left( \frac{1}{4} \right)}{2\sqrt{ \pi }}
}
$$

$$
\int_{0}^{\pi/2} \frac{1}{\sqrt{ \sin x }} \, \mathrm{d}x =
\frac{\Gamma\left( \frac{1}{4} \right)\Gamma\left( \frac{1}{2} \right)}{2\Gamma\left( \frac{3}{4} \right)} 
$$
$$
\boxed{
\int_{0}^{\pi/2} \frac{1}{\sqrt{ \sin x }} \, \mathrm{d}x =
\int_{0}^{\pi/2} \frac{1}{\sqrt{ \cos x }} \, \mathrm{d}x =
= \frac{\Gamma^{2}\left( \frac{1}{4} \right)}{2\sqrt{ 2\pi }}
} 
$$
%% todo %% pp127 v1

### x=y/(1+y)
4:2:1
$$
B(m,n) = \int_{0}^{1} x^{m-1}(1-x)^{n-1} \, \mathrm{d}x
, m>0, n>0
$$

make the change of vaiable 
${x=\frac{y}{1+y}}$ and so ${1-x = \frac{1}{1+y}}$
${dx = \frac{1}{(1+y)^{2}}dy}$
$$
B(m,n) 
= \int_{0}^{\infty} \left( \frac{y}{1+y} \right)^{m-1} \left( \frac{1}{1+y} \right)^{m-1} \frac{1}{(1+y)^{2}} \, \mathrm{d}y
= \int_{0}^{\infty} \frac{y^{m-1}}{(1+y)^{m+n}} \, \mathrm{d}y 
$$

setting ${n=1-m}$ 
$$
\int_{0}^{\infty} \frac{y^{m-1}}{1+y} \, \mathrm{d}x =
B(m,1-m) = \Gamma(m)\Gamma(1-m)
$$

using contour integration 8:7:9
$$
\int_{0}^{\infty} \frac{y^{m-1}}{1+y} \, \mathrm{d}y 
= \frac{\pi}{\sin(m \pi)}
$$

and so 
$$
\boxed{
\Gamma(m)\Gamma(1-m) = \frac{\pi}{\sin (m\pi)}
} 
$$
*reflection formula* for the gamma function, discovered by Euler in 1771.


### pp160 v2
from 4:2:5
$$
B(m,n) = \frac{\Gamma(m)\Gamma(n)}{\Gamma(m+n)}
= \frac{(m-1)!(n-1)!}{(m+n-1)!}
$$

from which it follows that
$$
B(m+1,n+1) = \frac{m!n!}{(m+n+1)!}
$$
let ${m=n=z}$, we have
$$
B(z+1,z+1) = 
\frac{z!z!}{(2z+1)!}
$$
by def
$$
B(z+1,z+1) = 
\int_{0}^{1} x^{z}(1-x)^{z} \, \mathrm{d}x 
$$

$$
\frac{z!z!}{(2z+1)!} = 
\int_{0}^{1} x^{z}(1-x)^{z} \, \mathrm{d}x 
$$

${x=\frac{1+s}{2}, 1-x = \frac{1-s}{2}, dx = \frac{1}{2}ds}$
$$
\frac{z!z!}{(2z+1)!} = 
\int_{-1}^{1} \left( \frac{1+s}{2} \right)^{z}\left( \frac{1-s}{2} \right)^{z} \frac{1}{2}\, \mathrm{d}s
= 2^{-2z-1} \int_{-1}^{1} (1-s^{2})^{z}  \, \mathrm{d}s 
$$

since the integrand is even
$$
\frac{z!z!}{(2z+1)!} = 
2^{-2z}\int_{0}^{1} (1-s^{2})^{z} \, \mathrm{d}s 
$$
let ${u=s^{2}, ds = \frac{1}{2\sqrt{ u }}du}$
$$
\frac{z!z!}{(2z+1)!} = 
2^{-2z}\int_{0}^{1} (1-u)^{z} \frac{1}{2\sqrt{ u }}  \, \mathrm{d}u 
$$

the last integral from 4:2:1
$$
B\left( \frac{1}{2}, z+1 \right) = 
\frac{\Gamma\left( \frac{1}{2} \right)\Gamma(z+1)}{\Gamma\left( z+\frac{3}{2} \right)}
= \frac{{\left( -\frac{1}{2} \right)!z!}}{\left( z+\frac{1}{2} \right)!}
$$

recalling from 4:2:11 ${\left( -\frac{1}{2} \right)! = \sqrt{ \pi }}$
$$
\frac{z!z!}{(2z+1)!} = 
2^{-2z-1} \frac{z!\sqrt{ \pi }}{\left( z+\frac{1}{2} \right)!}
$$

4:2:17
$$
z!\left( z+\frac{1}{2} \right)! = 2^{-2z-1}\sqrt{ \pi } (2z+1)!
$$

and since
${\left( z+\frac{1}{2} \right)! = \left( z+\frac{1}{2} \right) \left( z-\frac{1}{2} \right)! = \left( \frac{2z+1}{2} \right) \left( z-\frac{1}{2} \right)!}$
${(2z+1)! = (2z+1)(2z)!}$

4:2:18
$$
z!\left( z-\frac{1}{2} \right)! = 
2^{-2z}\sqrt{ \pi } (2z)!
$$





