
$$
I = \int_{0}^{\infty} \frac{\sin x}{x} \, \mathrm{d}x 
$$

$$
I = \frac{1}{2} 
\int_{-\infty }^{\infty} \frac{\sin x}{x} \, \mathrm{d}x 
$$
$$
F(a) = 
\int_{0}^{\infty} \frac{\sin x}{x} e^{ -ax } \, \mathrm{d}x 
$$
$$
F'(a) = 
\int_{0}^{\infty} \frac{\sin x}{x} e^{ -ax }(-x)\, \mathrm{d}x 
= -\int_{0}^{\infty} \sin{x} e^{ -ax }\, \mathrm{d}x 
$$
${ e^{ -ix } = \cos x+i\sin x }$ 
$$
F'(a) = -\mathrm{Im} \left( \int_{0}^{\infty} e^{ (i-a)x } \, \mathrm{d}x  \right)
= -\mathrm{Im}\left( \frac{1}{a-i} \right) = -\frac{1}{a^{2}+1}
$$
$$
F(a) = -\arctan a + C
$$
$$
F(+\infty ) = -\frac{\pi}{2}+C = 0, C = \frac{\pi}{2}
$$
$$
I = F(0) = \frac{\pi}{2}
$$



#### ex 1

$$
\int_{0}^{\infty}  \frac{\sin^{2}x}{x^{2}} \, \mathrm{d}x 
$$

$$
I = -\frac{1}{x}\sin ^{2}x \bigg|_{0}^{ \infty  } + \int_{0}^{\infty} \frac{1}{x} 2\sin x\cos x \, \mathrm{d}x 
$$
$$
I = 0 + \int_{0}^{\infty} \frac{\sin{2}x}{x} \, \mathrm{d}x 
$$

换元！
$$
I = \int_{0}^{\infty} \frac{\sin 2x}{2x} \, \mathrm{d}2x  = \frac{\pi}{2}
$$


#### ex 2
$$
\int_{0}^{\infty} \frac{\sin ^{3}x}{x^{3}} \, \mathrm{d}x 
$$

$$
F(k) = \int_{0}^{\infty} \frac{\sin ^{3}kx}{x^{3}} \, \mathrm{d}x 
$$
$$
F'(k) = \int_{0}^{\infty} \frac{3\sin ^{2}kx \cos kx \cdot x}{x^{3}} \, \mathrm{d}x 
$$
${ 3\sin ^{2}kx\cos kx = 3\cos kx - 3\cos ^{3}kx }$ 

${ \cos 3kx + i \sin 3kx = e^{ i 3k } = (e^{ ik })^{3} = (\cos kx + i\sin kx)^{3} }$ 
${ \cos 3kx = \cos ^{3}kx - 3\cos kx\sin ^{2}kx = 4\cos ^{3}kx - 3\cos kx }$ 
${ \cos ^{3}kx = \frac{1}{4}(\cos 3kx + 3\cos kx) }$ 

${ 3\cos kx - 3\cos ^{3}kx = 3 \cos kx - \frac{3}{4}(\cos 3kx - 3\cos kx) = \frac{3}{4}(\cos kx - \cos 3kx) }$ 

$$
F'(k) = \int_{0}^{\infty} \frac{-\frac{3}{4}\cos 3kx + \frac{3}{4}\cos kx}{x^{2}} \, \mathrm{d}x 
= \int_{0}^{\infty} -\frac{3}{4} \frac{\cos 3kx}{x^{2}} + \frac{3}{4} \frac{\cos kx}{x^{2}}\, \mathrm{d}x 
$$

$$
F''(k) = \int_{0}^{\infty} \frac{9}{4} \frac{\sin 3kx}{x} - \frac{3}{4} \frac{\sin kx}{x} \, \mathrm{d}x  = 
\frac{9}{4} \frac{\pi}{2} - \frac{3}{4} \frac{\pi}{2} = \frac{3\pi}{4}
$$

$$
F'(k) = \frac{3\pi}{4}k + C, F'(0) = 0,C =0
$$
$$
F(k) = \frac{3\pi}{8}k^{2} + C, F(0) = 0,C=0
$$
$$
I = F(1) = \frac{3\pi}{8}
$$

