
题目
$$
a,b,c>0,a+b+c= 3
$$
$$
\frac{1}{a^{2}} + 
\frac{1}{b^{2}} + 
\frac{1}{c^{2}} \geq
a^{2}+b^{2}+c^{2}
$$

## Answer by perplexity.ai/

To prove the inequality $(a^2 + b^2 + c^2 \leq \frac{1}{a^2} + \frac{1}{b^2} + \frac{1}{c^2})$ given that (a + b + c = 3) and (a, b, c > 0), we can use the Cauchy-Schwarz inequality.
However, the search results did not provide a direct Mathematica code for this specific inequality. Therefore, I will provide the proof using the Cauchy-Schwarz inequality. 

The Cauchy-Schwarz inequality states that for any real numbers $(x_1, x_2, ..., x_n)$ and $(y_1, y_2, ..., y_n)$, 
the following inequality holds: 
$$
(x_1^2 + x_2^2 + ... + x_n^2)(y_1^2 + y_2^2 + ... + y_n^2) \geq (x_1y_1 + x_2y_2 + ... + x_ny_n)^2
$$

We can use this inequality with $(x_1 = a, x_2 = b, x_3 = c, y_1 = \frac{1}{a}, y_2 = \frac{1}{b}, y_3 = \frac{1}{c})$ to prove the given inequality. 
By applying the Cauchy-Schwarz inequality, we have: 
$$(a^2 + b^2 + c^2)\left(\frac{1}{a^2} + \frac{1}{b^2} + \frac{1}{c^2}\right) \geq \left(a\cdot\frac{1}{a} + b\cdot\frac{1}{b} + c\cdot\frac{1}{c}\right)^2$$  
$$(a^2 + b^2 + c^2)\left(\frac{1}{a^2} + \frac{1}{b^2} + \frac{1}{c^2}\right) \geq (1 + 1 + 1)^2$$
$$(a^2 + b^2 + c^2)\left(\frac{1}{a^2} + \frac{1}{b^2} + \frac{1}{c^2}\right) \geq 3^2$$
$$(a^2 + b^2 + c^2)\left(\frac{1}{a^2} + \frac{1}{b^2} + \frac{1}{c^2}\right) \geq 9$$

Therefore, we have proved that: 
$$a^2 + b^2 + c^2 \leq \frac{1}{a^2} + \frac{1}{b^2} + \frac{1}{c^2}$$

This proof demonstrates that the inequality holds using the Cauchy-Schwarz inequality. 
While the direct Mathematica code for this specific inequality was not found in the search results, the proof using the Cauchy-Schwarz inequality establishes the validity of the given inequality.

---


https://www.bilibili.com/video/BV1gz4y1872i


切比雪夫不等式

$$
\begin{cases}
a_{1} \leq a_{2} \leq\dots \leq a_{n} \\
b_{1} \leq b_{2} \leq\dots \leq b_{n}
\end{cases}
$$

$$
a_{1}b_{1} + a_{2}b_{2} + \dots + a_{n}b_{n} 
\geq \frac{1}{n}\left( \sum_{j = 1}^{n} a_{j} \right)\left( \sum_{k = 1}^{n} b_{k} \right)
\geq
a_{1}b_{n} + a_{2}b_{n-1} + \dots + a_{n}b_{1} 
$$

正序大于乱序大于逆序

切比雪夫联合技术
有题设条件 ${ \sum a_{i}x_{i} \geq 0 }$ 
想证明 ${ \sum \frac{x_{i}}{y_{i}} \geq 0 }$ 

$$
a+b+c =3 \implies  \sum (a-1) = 0
$$
$$
\sum \frac{1}{a^{2}} \geq \sum a^{2} \implies 
\sum \frac{ 1-a^{ 4 } }{ a^{2} } = 
\sum (1-a)\left( \frac{ 1}{ a^{2} }  + \frac{1}{a} + 1 + a \right) \geq 0 
$$
不妨设 ${ a\geq b\geq c }$ 
如果 ${ a+1 + \frac{1}{a} + \frac{1}{a^{2}} \leq b + 1 + \frac{1}{b} + \frac{1}{b^{2}} }$ 即可
该式等价于 ${ (a-b)\left( -1 + \frac{1}{ab} + \frac{ a+b }{ a^{2}b^{2} } \right) \geq 0 }$ 

也就是 ${ a + b + ab \geq a^{2}b^{2} \Leftarrow 2\sqrt{ ab } + ab \geq a^{2}b^{2} }$ 
$$
f(x) = x^{ 4 } - x^{2} - 2x , x>1 \text{ 单调递增}
$$
作者是 ${ f(x) = x^{ 3 } - x - 2 , x>\frac{1}{\sqrt{ 3 }} \text{ 单调递增} }$ 


$$
\sqrt{ ab } = \sqrt{ a(3-a-c) } < \sqrt{ a(3-a) } < \frac{3}{2}, 
f(x) < f\left( \frac{3}{2} \right) < 0
$$
