$$
(1 + Az + Bz^{2} + Cz^{3} + Dz^{4} + \dots) = (1 + \alpha z)(1 + \beta z)(1 + \gamma z)(1 + \delta z)\dots
$$

$$
\begin{align}
A & = \alpha + \beta + \gamma + \delta + \dots \\
B & = \alpha\beta + \alpha\gamma + \alpha\delta + \beta\gamma + \beta\delta + \gamma\delta \dots \\
C & = \alpha\beta\gamma + \alpha\beta\delta + \beta\gamma\delta + \dots
\end{align}
$$

$$
\begin{align}
P & = \alpha+\beta+\gamma+\delta+\varepsilon+\cdots \\
Q & = \alpha^{2}+\beta^{2}+\gamma^{2}+\delta^{2}+\varepsilon^{2}+\cdots \\
R & = \alpha^{3}+\beta^{3}+\gamma^{3}+\delta^{3}+\varepsilon^{3}+\cdots \\
S & = \alpha^{4}+\beta^{4}+\gamma^{4}+\delta^{4}+\varepsilon^{4}+\cdots \\
T & = \alpha^{5}+\beta^{5}+\gamma^{5}+\delta^{5}+\varepsilon^{5}+\cdots \\
V & = \alpha^{6}+\beta^{6}+\gamma^{6}+\delta^{6}+\varepsilon^{6}+\cdots
\end{align}
$$

$$
\begin{align}
P & = A \\
Q & = A P-2 B \\
R & = A Q-B P+3 C \\
S & = A R-B Q+C P-4 D \\
T & = A S-B R+C Q-D P+5 E \\
V & = A T-B S+C R-D Q+E P-6 F \\
\end{align}
$$
可以直观地想象这些公式, 并验证它们成立, 严格的证明由微积分学给出.

Sec 167 
$$
\frac{e^{x} - e^{-x}}{2}
= x + \frac{x^{3}}{3!} + \frac{x^{5}}{5!} + \dots 
= x\left( 1 + \frac{x^{2}}{\pi^{2}} \right)\left( 1 + \frac{x^{2}}{4\pi^{2}} \right)\left( 1+\frac{x^{2}}{9\pi^{2}} \right) \dots
$$
$$ 1 + \frac{x^{2}}{3!} + \frac{x^{4}}{5!} + \dots = \left( 1 + \frac{x^{2}}{\pi^{2}} \right)\left( 1 + \frac{x^{2}}{4\pi^{2}} \right)\left( 1+\frac{x^{2}}{9\pi^{2}} \right) \dots $$
let ${x^{2} = \pi^{2}z}$
$$ 1 + \frac{\pi^{2}z}{3!} + \frac{\pi^{4}z^{2}}{5!} + \dots = \left( 1 + z \right)\left( 1 + \frac{z}{4} \right)\left( 1+\frac{z}{9} \right) \dots $$

$$
A =  \frac{\pi^{2}}{6}, B = \frac{\pi^{4}}{120}, C = \frac{\pi^{6}}{5040}, D = \frac{\pi^{8}}{362880}
$$
$$
\begin{align}
P & = 1 + \frac{1}{4} + \frac{1}{9} + \dots \\
Q & = 1 + \frac{1}{4^{2}} + \frac{1}{9^{2}} + \dots \\
R & = 1 + \frac{1}{4^{3}} + \frac{1}{9^{3}} + \dots
\end{align}
$$


$$
\begin{align}
P & = A   & = \frac{\pi^{2}}{6}\\
Q & = A P-2 B = \frac{\pi^{2}}{6}\times  \frac{\pi^{2}}{6} - 2 \times \frac{\pi^{4}}{120}  & = \frac{\pi^{4}}{90}\\
R & = A Q-B P+3 C = \frac{\pi^{2}}{6} \times \frac{\pi^{4}}{90} - \frac{\pi^{4}}{120}\times \frac{\pi^{2}}{6} + 3\times \frac{\pi^{6}}{5040} & = \frac{\pi^{6}}{945} \\
S & = A R-B Q+C P-4 D = \frac{\pi^{2}}{6} \times \frac{\pi^{6}}{945} - \frac{\pi^{4}}{120}\times \frac{\pi^{4}}{90} + \frac{\pi^{6}}{5040} \times \frac{\pi^{2}}{6} - 4\times  \frac{\pi^{8}}{362880} & =\frac{\pi^{8}}{9450} \\
T & = A S-B R+C Q-D P+5 E  & = \frac{\pi^{10}}{93555}\\
\end{align}
$$

```mathematica
In[1]:= 1/6/90 - 1/120/6 + 3/5040
Out[1]= 1/945
In[2]:= 1/6/945 - 1/120/90 + 1/5040/6 - 4/362880
Out[2]= 1/9450
In[3]:= 1/6/9450 - 1/120/945 + 1/5040/90 - 1/362880/6 + 5/39916800
Out[3]= 1/93555
```

%% todo %%
