1 ${ x = (X_{L}, X_{R}), X_{L} \ngeq X_{R} }$ 
2 ${ x \leq y \implies X_{L} \ngeq y \;\&\; x \ngeq Y_{R} }$ 
3 加法 ${ x+y = ((X_{L} + y)\cup (Y_{L} + x), (X_{R}+y)\cup (Y_{R} + x)) }$ 
4 逆元 ${ -x = (-X_{R}, -X_{L}) }$ 

T1 保序性 ${ x \leq y, y \leq z \implies x \leq z }$ 
T2 ${ X_{L} \leq x \;\&\; x \leq X_{R} }$ 
T3 自反性 ${ x \leq x }$ 
T4 ${ x \nleq y \implies y \leq x }$ 
T5 传递律 ${ x<y, y\leq z \implies x<z }$ 
T6 传递律 ${ x\leq y, y< z \implies x<z }$ 
T7 ${ Y_{L}<x<Y_{R} \implies x \equiv (X_{L}\cup Y_{L}, X_{R}\cup Y_{R}) }$ 
T8 ${ \forall y = (Y_{L}, Y_{R}) }$， ${ x }$ 是创造出来的数中首个满足${ Y_{L}<x, x<Y_{R} }$ 的数，则有${ x \equiv y }$  
T9 ${ x+y = y+x }$ 
T10 ${ x+0 = x }$ 

