
https://zhuanlan.zhihu.com/p/299011986

$$
1-\frac{1}{3} + \frac{1}{5} - \frac{1}{7} + \dots = \frac{\pi}{4}
$$


等比数列 Geometric sequence 
$$
1+x+x^{2}+x^{3} +x^{4} + \dots +x^{n}= \frac{1-x^{n+1}}{1-x}
$$
${\left| x \right|<1}$ 
$$
1+x+x^{2}+x^{3} +x^{4} + \dots = \frac{1}{1-x}
$$

$$
\int_{0}^{x} \frac{1}{1+t^{2}} \, \mathrm{d}t = \arctan t\Bigg|_{0}^{x} = \arctan x  
$$
$$
\int_{0}^{x} \frac{1}{1+t^{2}}  \, \mathrm{d}t =
\int_{0}^{x} 1+(-t^{2})+(-t^{2})^{2}+(-t^{2})^{3}+,,,  \, \mathrm{d}t =
x-\frac{1}{3}s^{3} + \frac{1}{5}x^{5}-\dots
$$
${x=1}$
$$
\frac{\pi}{4} = 1-\frac{1}{3}+\frac{1}{5}-\frac{1}{7}+\dots
$$


## Ex
2717-BMT-Analysis-07

Compute 
$$
\sum_{k = 1}^{\infty} \frac{(-1)^{k}}{(2k-1)(2k+1)}
$$

$$
\frac{(-1)^{k}}{(2k-1)(2k+1)} = \frac{(-1)^{k}}{2} \left( \frac{1}{2k-1} - \frac{1}{2k+1} \right) 
$$
$$
I = \frac{1}{2} 
\sum_{k = 1}^{\infty} \left( 
\frac{(-1)^{k}}{2k-1} - 
\frac{(-1)^{k}}{2k+1}
\right)
$$
$$
I = \frac{1}{2} \left( \left( -1+\frac{1}{3}-\frac{1}{5}+\dots \right) - \left( -\frac{1}{3} + \frac{1}{5}-\frac{1}{7} \right)\right)
$$
$$
I = \frac{1}{2}\left( -\frac{\pi}{4} - \left( \frac{\pi}{4}-1 \right) \right)
$$
$$
I = \frac{1}{2} - \frac{\pi}{4}
$$

